Add decr_loop examples

nola/examples/basic.v
@@ -8,10 +8,14 @@ Import ModwNotation WpwNotation CsemNotation.
 Definition just_loop : val := rec: "self" ["n"] :=
   if:: "n" > #0 then "self" ["n" - #1].
 
+(** Loop decrementing the value of a location *)
+Definition decr_loop : val := rec: "self" ["l"] :=
+  if:: !"l" > #0 then "l" <- !"l" - #1;; "self" ["l"].
+
 Section basic.
   Context `{!lrustGS_gen hlc Σ}.
 
-  (** [just_loop] terminates for any non-negative [n] *)
+  (** [just_loop] terminates for any [n] *)
   Lemma twp_just_loop {W E} {n : nat} :
     [[{ True }]][W] just_loop [ #n] @ E [[{ RET #☠; True }]].
   Proof.
@@ -20,12 +24,31 @@ Section basic.
     wp_op. have ->: (S n - 1)%Z = n by lia. by iApply "IH".
   Qed.
 
-  (** [just_loop] called with [Ndnat] *)
+  (** [just_loop] called with a non-deterministic input *)
   Lemma twp_just_loop_nd {W E} :
     [[{ True }]][W] just_loop [Ndnat] @ E [[{ RET #☠; True }]].
   Proof.
     iIntros (?) "_ →Φ". wp_apply twp_ndnat=>//. iIntros (?) "_".
     by wp_apply twp_just_loop.
+  Qed.
+
+  (** [decr_loop] terminates for any [n] *)
+  Lemma twp_decr_loop {W E l} {n : nat} :
+    [[{ l ↦ #n }]][W] decr_loop [ #l] @ E [[{ RET #☠; l ↦ #0 }]].
+  Proof.
+    iIntros (?) "↦ →Φ".
+    iInduction n as [|n] "IH"; wp_rec; wp_read; wp_op; wp_case;
+      [by iApply "→Φ"|].
+    wp_read. wp_op. wp_write. have ->: (S n - 1)%Z = n by lia.
+    iApply ("IH" with "↦ →Φ").
+  Qed.
+
+  (** [decr_loop] called with non-deterministic initialization *)
+  Lemma twp_decr_loop_nd {W E l v} :
+    [[{ l ↦ v }]][W] #l <- Ndnat;; decr_loop [ #l] @ E [[{ RET #☠; l ↦ #0 }]].
+  Proof.
+    iIntros (?) "↦ →Φ". wp_apply twp_ndnat=>//. iIntros (?) "_". wp_write.
+    wp_apply (twp_decr_loop with "↦ →Φ").
   Qed.
 
   Context `{!Csem CON JUDG Σ, !Jsem JUDG (iProp Σ), !inv'GS (cifOF CON) Σ,
@@ -34,10 +57,21 @@ Section basic.
   (** [just_loop] called with a value taken from an invariant *)
   Lemma twp_just_loop_inv {N E l} : ↑N ⊆ E →
     [[{ inv_tok N (∃ n : nat, ▷ l ↦ #n)%cif }]][inv_wsat ⟦⟧ᶜ]
-      just_loop [(!ˢᶜ#l)] @ E [[{ RET #☠; True }]].
+      just_loop [!ˢᶜ #l] @ E [[{ RET #☠; True }]].
   Proof.
-    iIntros (??) "#i →Φ". wp_bind (!ˢᶜ_)%E.
+    iIntros (??) "#i →Φ". wp_bind (!ˢᶜ _)%E.
     iMod (inv_tok_acc with "i") as "/=[[% >↦] cl]"=>//. wp_read.
     iMod ("cl" with "[$↦]"). iModIntro. by wp_apply twp_just_loop.
+  Qed.
+
+  (** [decr_loop] called with a value taken from an invariant *)
+  Lemma twp_decr_loop_inv {N E l l' v} : ↑N ⊆ E →
+    [[{ inv_tok N (∃ n : nat, ▷ l' ↦ #n)%cif ∗ l ↦ v }]][inv_wsat ⟦⟧ᶜ]
+      #l <- !ˢᶜ #l';; decr_loop [ #l] @ E [[{ RET #☠; l ↦ #0 }]].
+  Proof.
+    iIntros (??) "[#i ↦] →Φ". wp_bind (!ˢᶜ _)%E.
+    iMod (inv_tok_acc with "i") as "/=[[% >↦'] cl]"=>//. wp_read.
+    iMod ("cl" with "[$↦']"). iModIntro. wp_write.
+    wp_apply (twp_decr_loop with "↦ →Φ").
   Qed.
 End basic.
